theories/c_interop/rules.v
@@ -22,11 +22,11 @@ Context `{!wrapperGCtokG Σ}.
 
 (* Reading and writing roots using plain C reads and writes *)
 
-Lemma store_to_root pe (l:loc) (v v' : lval) w θ :
+Lemma store_to_root pe (l:loc) (v v' : lval) w θ dirty :
   repr_lval θ v w →
-  {{{ GC θ ∗ l ↦roots v' }}}
+  {{{ GC θ dirty ∗ l ↦roots v' }}}
      (#l <- w)%CE at pe
-  {{{ RET LitV LitUnit; GC θ ∗ l ↦roots v }}}%CE.
+  {{{ RET LitV LitUnit; GC θ dirty ∗ l ↦roots v }}}%CE.
 Proof.
   iIntros (Hrepr Φ) "(HGC&Hroot) HΦ".
   iDestruct (update_root with "[$HGC $Hroot]") as (w') "(Hpto & _ & Hupd)".
@@ -36,10 +36,10 @@ Proof.
   iApply "HΦ". by iFrame.
 Qed.
 
-Lemma load_from_root pe (l:loc) (v : lval) dq θ :
-  {{{ GC θ ∗ l ↦roots{dq} v }}}
+Lemma load_from_root pe (l:loc) (v : lval) dq θ dirty :
+  {{{ GC θ dirty ∗ l ↦roots{dq} v }}}
      ( * #l)%CE at pe
-  {{{ w, RET w; l ↦roots{dq} v ∗ GC θ ∗ ⌜repr_lval θ v w⌝ }}}%CE.
+  {{{ w, RET w; l ↦roots{dq} v ∗ GC θ dirty ∗ ⌜repr_lval θ v w⌝ }}}%CE.
 Proof.
   iIntros (Φ) "(HGC&Hroot) HΦ".
   iDestruct (access_root with "[$HGC $Hroot]") as (w') "(Hpto & %Hrepr & Hupd)".
@@ -49,99 +49,99 @@ Qed.
 
 (* Calling to runtime primitives *)
 
-Lemma wp_int2val p Ψ θ (x : Z) :
+Lemma wp_int2val p Ψ θ dirty (x : Z) :
   p !! "int2val" = None →
   int2val_proto ⊑ Ψ →
-  {{{ GC θ }}}
+  {{{ GC θ dirty }}}
     (call: &"int2val" with (Val #x))%CE at ⟨p, Ψ⟩
-  {{{ w, RET w; GC θ ∗ ⌜repr_lval θ (Lint x) w⌝ }}}.
+  {{{ w, RET w; GC θ dirty ∗ ⌜repr_lval θ (Lint x) w⌝ }}}.
 Proof.
   iIntros (Hp Hproto Φ) "HGC Cont".
   wp_pures. wp_extern; first done.
   iModIntro. cbn. iApply Hproto.
-  rewrite /int2val_proto /named. iExists _, _. iFrame.
+  rewrite /int2val_proto /named. iExists _, _, _. iFrame.
   do 2 (iSplit; first by eauto). iIntros "!>" (?) "HGC %".
   iApply wp_value; eauto. iApply "Cont"; eauto.
 Qed.
 
-Lemma wp_val2int p Ψ θ (w:word) (x : Z) :
+Lemma wp_val2int p Ψ θ dirty (w:word) (x : Z) :
   p !! "val2int" = None →
   val2int_proto ⊑ Ψ →
   repr_lval θ (Lint x) w →
-  {{{ GC θ }}}
+  {{{ GC θ dirty }}}
     (call: &"val2int" with (Val w))%CE at ⟨p, Ψ⟩
-  {{{ RET (#x); GC θ }}}.
+  {{{ RET (#x); GC θ dirty }}}.
 Proof.
   iIntros (Hp Hproto Hrepr Φ) "HGC Cont".
   wp_pures. wp_extern; first done.
   iModIntro. cbn. iApply Hproto.
-  rewrite /val2int_proto /named. iExists _, _, _. iFrame.
+  rewrite /val2int_proto /named. iExists _, _, _, _. iFrame.
   do 3 (iSplit; first by eauto). iIntros "!> HGC".
   iApply wp_value; eauto. iApply "Cont"; eauto.
 Qed.
 
-Lemma wp_registerroot p Ψ θ v w a :
+Lemma wp_registerroot p Ψ θ dirty v w a :
   p !! "registerroot" = None →
   registerroot_proto ⊑ Ψ →
   repr_lval θ v w →
-  {{{ GC θ ∗ a ↦C w }}}
+  {{{ GC θ dirty ∗ a ↦C w }}}
     (call: &"registerroot" with (Val (# a)))%CE at ⟨p, Ψ⟩
-  {{{ RET (# 0); GC θ ∗ a ↦roots v }}}.
+  {{{ RET (# 0); GC θ dirty ∗ a ↦roots v }}}.
 Proof.
   iIntros (Hp Hproto Hrepr Φ) "(HGC & Hpto) Cont".
   wp_pures. wp_extern; first done.
   iModIntro. cbn. iApply Hproto.
   rewrite /registerroot_proto /named.
-  iExists _, _, _, _. iFrame.
+  iExists _, _, _, _, _. iFrame.
   do 3 (iSplit; first by eauto). iIntros "!> ? ?".
   iApply wp_value; eauto. iApply "Cont"; eauto. iFrame.
 Qed.
 
-Lemma wp_unregisterroot p Ψ θ v a :
+Lemma wp_unregisterroot p Ψ θ dirty v a :
   p !! "unregisterroot" = None →
   unregisterroot_proto ⊑ Ψ →
-  {{{ GC θ ∗ a ↦roots v }}}
+  {{{ GC θ dirty ∗ a ↦roots v }}}
     (call: &"unregisterroot" with (Val (# a)))%CE at ⟨p, Ψ⟩
-  {{{ w, RET (# 0); GC θ ∗ a ↦C w ∗ ⌜repr_lval θ v w⌝ }}}.
+  {{{ w, RET (# 0); GC θ dirty ∗ a ↦C w ∗ ⌜repr_lval θ v w⌝ }}}.
 Proof.
   iIntros (Hp Hproto Φ) "(HGC & Hpto) Cont".
   wp_pures. wp_extern; first done.
   iModIntro. cbn. iApply Hproto.
   rewrite /unregisterroot_proto /named.
-  iExists _, _, _. iFrame.
+  iExists _, _, _, _. iFrame.
   do 2 (iSplit; first by eauto). iIntros "!>" (?) "? ? %".
   iApply wp_value; eauto. iApply "Cont"; eauto. by iFrame.
 Qed.
 
-Lemma wp_modify p Ψ θ γ w mut tg vs v' w' i :
+Lemma wp_modify p Ψ θ dirty γ w mut tg vs v' w' i :
   p !! "modify" = None →
   modify_proto ⊑ Ψ →
   repr_lval θ (Lloc γ) w →
   vblock_access_le M mut →
   repr_lval θ v' w' →
   (0 ≤ i < length vs)%Z →
-  {{{ GC θ ∗ γ ↦vblk[mut] (tg, vs) }}}
+  {{{ GC θ dirty ∗ γ ↦vblk[mut] (tg, vs) }}}
     (call: &"modify" with (Val w, Val (# i), Val w'))%CE at ⟨p, Ψ⟩
-  {{{ RET (# 0); GC θ ∗ γ ↦vblk[mut] (tg, <[Z.to_nat i:=v']> vs) }}}.
+  {{{ RET (# 0); GC θ dirty ∗ γ ↦vblk[mut] (tg, <[Z.to_nat i:=v']> vs) }}}.
 Proof.
   intros Hp Hproto **. iIntros "(HGC & Hpto) Cont".
   wp_pures. wp_extern; first done.
   iModIntro. cbn. iApply Hproto.
   rewrite /modify_proto /named.
-  do 9 iExists _. iFrame.
+  do 10 iExists _. iFrame.
   do 7 (iSplit; first by eauto with lia). iIntros "!> ? ?".
   iApply wp_value; eauto. iApply "Cont"; eauto. by iFrame.
 Qed.
 
-Lemma wp_readfield p Ψ θ γ w m dq tg vs i :
+Lemma wp_readfield p Ψ θ dirty γ w m dq tg vs i :
   p !! "readfield" = None →
   readfield_proto ⊑ Ψ →
   repr_lval θ (Lloc γ) w →
   (0 ≤ i < length vs)%Z →
-  {{{ GC θ ∗ γ ↦vblk[m]{dq} (tg, vs) }}}
+  {{{ GC θ dirty ∗ γ ↦vblk[m]{dq} (tg, vs) }}}
     (call: &"readfield" with (Val w, Val (# i)))%CE at ⟨p, Ψ⟩
   {{{ v' w', RET w';
-        GC θ ∗ γ ↦vblk[m]{dq} (tg, vs) ∗
+        GC θ dirty ∗ γ ↦vblk[m]{dq} (tg, vs) ∗
         ⌜vs !! (Z.to_nat i) = Some v'⌝ ∗
         ⌜repr_lval θ v' w'⌝ }}}.
 Proof.
@@ -149,159 +149,159 @@ Proof.
   wp_pures. wp_extern; first done.
   iModIntro. cbn. iApply Hproto.
   rewrite /readfield_proto /named.
-  do 8 iExists _. iFrame.
+  do 9 iExists _. iFrame.
   do 5 (iSplit; first by eauto with lia). iIntros "!>" (? ?) "? ?".
   iIntros (? ?).
   iApply wp_value; eauto. iApply "Cont"; eauto. by iFrame.
 Qed.
 
-Lemma wp_isblock p Ψ θ lv w :
+Lemma wp_isblock p Ψ θ dirty lv w :
   p !! "isblock" = None →
   isblock_proto ⊑ Ψ →
   repr_lval θ lv w →
-  {{{ GC θ }}}
+  {{{ GC θ dirty }}}
     (call: &"isblock" with (Val w))%CE at ⟨p, Ψ⟩
-  {{{ RET #(match lv return Z with | Lloc _ => 1 | _ => 0 end); GC θ }}}.
+  {{{ RET #(match lv return Z with | Lloc _ => 1 | _ => 0 end); GC θ dirty }}}.
 Proof.
   intros Hp Hproto **. iIntros "HGC Cont".
   wp_pures. wp_extern; first done.
   iModIntro. cbn. iApply Hproto.
   rewrite /isblock_proto /named.
-  do 3 iExists _. iFrame "HGC".
+  do 4 iExists _. iFrame "HGC".
   do 3 (iSplit; first done). iNext.
   iIntros "HGC". wp_pures. iApply ("Cont" with "HGC").
 Qed.
 
-Lemma wp_isblock_true p Ψ θ γ w :
+Lemma wp_isblock_true p Ψ θ dirty γ w :
   p !! "isblock" = None →
   isblock_proto ⊑ Ψ →
   repr_lval θ (Lloc γ) w →
-  {{{ GC θ }}}
+  {{{ GC θ dirty }}}
     (call: &"isblock" with (Val w))%CE at ⟨p, Ψ⟩
-  {{{ RET #1; GC θ }}}.
+  {{{ RET #1; GC θ dirty }}}.
 Proof.
   intros Hp Hproto **. iIntros "HGC Cont".
   iApply (wp_isblock with "HGC"); [done..|].
   iIntros "!> HGC". by iApply "Cont".
 Qed.
 
-Lemma wp_isblock_false p Ψ θ z w :
+Lemma wp_isblock_false p Ψ θ dirty z w :
   p !! "isblock" = None →
   isblock_proto ⊑ Ψ →
   repr_lval θ (Lint z) w →
-  {{{ GC θ }}}
+  {{{ GC θ dirty }}}
     (call: &"isblock" with (Val w))%CE at ⟨p, Ψ⟩
-  {{{ RET #0; GC θ }}}.
+  {{{ RET #0; GC θ dirty }}}.
 Proof.
   intros Hp Hproto **. iIntros "HGC Cont".
   iApply (wp_isblock with "HGC"); [done..|].
   iIntros "!> HGC". by iApply "Cont".
 Qed.
 
-Lemma wp_read_tag p Ψ θ γ w dq bl :
+Lemma wp_read_tag p Ψ θ dirty γ w dq bl :
   p !! "read_tag" = None →
   read_tag_proto ⊑ Ψ →
   repr_lval θ (Lloc γ) w →
-  {{{ GC θ ∗ lstore_own_elem γ dq bl}}}
+  {{{ GC θ dirty ∗ lstore_own_elem γ dq bl}}}
     (call: &"read_tag" with (Val w))%CE at ⟨p, Ψ⟩
-  {{{ RET #(tag_as_int (block_tag bl)); GC θ ∗ lstore_own_elem γ dq bl }}}.
+  {{{ RET #(tag_as_int (block_tag bl)); GC θ dirty ∗ lstore_own_elem γ dq bl }}}.
 Proof.
   intros Hp Hproto **. iIntros "(HGC&Hpto) Cont".
   wp_pures. wp_extern; first done.
   iModIntro. cbn. iApply Hproto.
   rewrite /read_tag_proto /named.
-  do 6 iExists _. iFrame "HGC Hpto".
+  do 7 iExists _. iFrame "HGC Hpto".
   do 4 (iSplit; first done). iNext.
   iIntros "HGC Hpto". wp_pures. iApply ("Cont" with "[$]").
 Qed.
 
-Lemma wp_length p Ψ θ γ w m dq tg vs :
+Lemma wp_length p Ψ θ dirty γ w m dq tg vs :
   p !! "length" = None →
   length_proto ⊑ Ψ →
   repr_lval θ (Lloc γ) w →
-  {{{ GC θ ∗ γ ↦vblk[m]{dq} (tg, vs) }}}
+  {{{ GC θ dirty ∗ γ ↦vblk[m]{dq} (tg, vs) }}}
     (call: &"length" with (Val w))%CE at ⟨p, Ψ⟩
   {{{ RET #(length vs);
-        GC θ ∗ γ ↦vblk[m]{dq} (tg, vs) }}}.
+        GC θ dirty ∗ γ ↦vblk[m]{dq} (tg, vs) }}}.
 Proof.
   intros Hp Hproto **. iIntros "(HGC & Hpto) Cont".
   wp_pures. wp_extern; first done.
   iModIntro. cbn. iApply Hproto.
   rewrite /length_proto /named.
-  do 6 iExists _. iFrame.
+  do 7 iExists _. iFrame.
   do 3 (iSplit; first by eauto with lia). iIntros "!> HGC Hpto".
   cbn.
   iApply wp_value; eauto. iApply "Cont"; eauto. by iFrame.
 Qed.
 
-Lemma wp_alloc tg p Ψ θ tgnum sz :
+Lemma wp_alloc tg p Ψ θ dirty tgnum sz :
   p !! "alloc" = None →
   alloc_proto ⊑ Ψ →
   (0 ≤ sz)%Z →
   vblock_tag_as_int tg = tgnum →
-  {{{ GC θ }}}
+  {{{ GC θ dirty }}}
     (call: &"alloc" with (Val (# tgnum), Val (# sz)))%CE at ⟨p, Ψ⟩
   {{{ θ' γ w, RET w;
-        GC θ' ∗ γ ↦fresh (tg, List.repeat (Lint 0) (Z.to_nat sz)) ∗
+        GC θ' dirty ∗ γ ↦fresh (tg, List.repeat (Lint 0) (Z.to_nat sz)) ∗
         ⌜repr_lval θ' (Lloc γ) w⌝ }}}.
 Proof.
   intros Hp Hproto **. iIntros "HGC Cont".
   wp_pures. wp_extern; first done.
   iModIntro. cbn. iApply Hproto.
   rewrite /alloc_proto /named.
-  do 3 iExists _. iFrame. subst.
+  do 4 iExists _. iFrame. subst.
   do 3 (iSplit; first by eauto with lia). iIntros "!>" (? ? ?) "? ? %".
   iApply wp_value; eauto. iApply "Cont"; eauto. by iFrame.
 Qed.
 
-Lemma wp_alloc_foreign p Ψ θ :
+Lemma wp_alloc_foreign p Ψ θ dirty :
   p !! "alloc_foreign" = None →
   alloc_foreign_proto ⊑ Ψ →
-  {{{ GC θ }}}
+  {{{ GC θ dirty }}}
     (call: &"alloc_foreign" with ( ))%CE at ⟨p, Ψ⟩
   {{{ θ' γ w, RET w;
-        GC θ' ∗ γ ↦foreignO None ∗
+        GC θ' dirty ∗ γ ↦foreignO None ∗
         ⌜repr_lval θ' (Lloc γ) w⌝ }}}.
 Proof.
   intros Hp Hproto **. iIntros "HGC Cont".
   wp_pures. wp_extern; first done.
   iModIntro. cbn. iApply Hproto.
   rewrite /alloc_foreign_proto /named.
-  do 1 iExists _. iFrame.
+  do 2 iExists _. iFrame.
   do 2 (iSplit; first by eauto). iIntros "!>" (? ? ?) "? ? %".
   iApply wp_value; eauto. iApply "Cont"; eauto. by iFrame.
 Qed.
 
-Lemma wp_write_foreign p Ψ θ w γ ao a' :
+Lemma wp_write_foreign p Ψ θ dirty w γ ao a' :
   p !! "write_foreign" = None →
   write_foreign_proto ⊑ Ψ →
   repr_lval θ (Lloc γ) w →
-  {{{ GC θ ∗ γ ↦foreignO ao }}}
+  {{{ GC θ dirty ∗ γ ↦foreignO ao }}}
     (call: &"write_foreign" with (Val w, Val a'))%CE at ⟨p, Ψ⟩
-  {{{ RET (# 0); GC θ ∗ γ ↦foreign a' }}}.
+  {{{ RET (# 0); GC θ dirty ∗ γ ↦foreign a' }}}.
 Proof.
   intros Hp Hproto **. iIntros "(HGC & ?) Cont".
   wp_pures. wp_extern; first done.
   iModIntro. cbn. iApply Hproto.
   rewrite /write_foreign_proto /named.
-  do 5 iExists _. iFrame.
+  do 6 iExists _. iFrame.
   do 3 (iSplit; first by eauto with lia). iIntros "!> ? ?".
   iApply wp_value; eauto. iApply "Cont"; eauto. by iFrame.
 Qed.
 
-Lemma wp_read_foreign p Ψ θ w γ a dq :
+Lemma wp_read_foreign p Ψ θ dirty w γ a dq :
   p !! "read_foreign" = None →
   read_foreign_proto ⊑ Ψ →
   repr_lval θ (Lloc γ) w →
-  {{{ GC θ ∗ γ ↦foreign{dq} a }}}
+  {{{ GC θ dirty ∗ γ ↦foreign{dq} a }}}
     (call: &"read_foreign" with (Val w))%CE at ⟨p, Ψ⟩
-  {{{ RET a; GC θ ∗ γ ↦foreign{dq} a }}}.
+  {{{ RET a; GC θ dirty ∗ γ ↦foreign{dq} a }}}.
 Proof.
   intros Hp Hproto **. iIntros "(HGC & ?) Cont".
   wp_pures. wp_extern; first done.
   iModIntro. cbn. iApply Hproto.
   rewrite /read_foreign_proto /named.
-  do 5 iExists _. iFrame.
+  do 6 iExists _. iFrame.
   do 3 (iSplit; first by eauto with lia). iIntros "!> ? ?".
   iApply wp_value; eauto. iApply "Cont"; eauto. by iFrame.
 Qed.
@@ -311,14 +311,14 @@ Lemma wp_callback p ΨML Ψ θ w γ f x e lv' w' v' Φ :
   callback_proto ΨML ⊑ Ψ →
   repr_lval θ (Lloc γ) w →
   repr_lval θ lv' w' →
-  {{{ GC θ ∗
+  {{{ GC θ ∅ ∗
       γ ↦clos (f, x, e) ∗
       lv' ~~ v' ∗
       (▷ WP (App (ML_lang.Val (RecV f x e)) (ML_lang.Val v')) at ⟨∅, ΨML⟩ {{ Φ }})
   }}}
     (call: &"callback" with (Val w, Val w'))%CE at ⟨p, Ψ⟩
   {{{ θ' vret lvret wret, RET wret;
-        GC θ' ∗
+        GC θ' ∅ ∗
         Φ vret ∗
         lvret ~~ vret ∗
         ⌜repr_lval θ' lvret wret⌝ }}}.
@@ -349,13 +349,13 @@ Proof.
 Qed.
 
 (* Macro Laws *)
-Lemma wp_CAMLlocal n e2 p Ψ Φ θ :
+Lemma wp_CAMLlocal n e2 p Ψ Φ θ dirty :
   p !! "int2val" = None →
   int2val_proto ⊑ Ψ →
   p !! "registerroot" = None →
   registerroot_proto ⊑ Ψ →
-  (⊢ GC θ -∗
-     (▷ ∀ (l:loc), GC θ ∗ l ↦roots Lint 0 -∗ WP (subst_all {[n := #l]} e2) at ⟨ p, Ψ ⟩ {{Φ}}) -∗
+  (⊢ GC θ dirty -∗
+     (▷ ∀ (l:loc), GC θ dirty ∗ l ↦roots Lint 0 -∗ WP (subst_all {[n := #l]} e2) at ⟨ p, Ψ ⟩ {{Φ}}) -∗
      WP (CAMLlocal: n in e2)%CE at ⟨ p, Ψ ⟩
      {{Φ}}%CE)%I.
 Proof.
@@ -371,12 +371,12 @@ Proof.
   iApply "Cont". iFrame.
 Qed.
 
-Lemma wp_CAMLunregister1 (l:loc) lv p θ Ψ :
+Lemma wp_CAMLunregister1 (l:loc) lv p θ dirty Ψ :
   p !! "unregisterroot" = None →
   unregisterroot_proto ⊑ Ψ →
-  {{{ GC θ ∗ l ↦roots lv}}}
+  {{{ GC θ dirty ∗ l ↦roots lv}}}
     (CAMLunregister1 (#l))%CE at ⟨p, Ψ⟩
-  {{{ RET (#0); GC θ }}}.
+  {{{ RET (#0); GC θ dirty }}}.
 Proof.
   iIntros (???) "Hin Cont".
   unfold CAMLunregister1.
