theories/interop/wp_prims/alloc.v
@@ -28,7 +28,7 @@ Proof using.
   iIntros (Φ') "Hb Hcont". iApply wp_wrap_call; first done. cbn [snd].
   rewrite weakestpre.wp_unfold. rewrite /weakestpre.wp_pre.
   iIntros "%σ Hσ". cbn -[wrap_prog].
-  SI_at_boundary. iNamed "HGC". SI_GC_agree.
+  SI_at_boundary. iNamed "HGC". SI_GC_agree. iNamed "HSI_GC". iNamed "HSI_block_level".
   pose (tg, repeat (Lint 0) (Z.to_nat sz)) as blk.
   iAssert (⌜∀ k lv, roots_m !! k = Some lv →
             ∃ w, mem !! k = Some (Storing w) ∧ repr_lval (θC ρc) lv w⌝)%I as "%Hroots".
@@ -46,8 +46,8 @@ Proof using.
     χC' = <[γ := LlocPrivate]> (χC ρc) ∧
     ζC' = <[γ := Bvblock (Mut, (tg, repeat (Lint 0) (Z.to_nat sz)))]> (ζC ρc) ∧
     GC_correct ζC' θC' ∧
-    repr θC' roots_m privmem mem' ∧
-    roots_are_live θC' roots_m ∧
+    repr θC' _ _ _ ∧
+    roots_are_live θC' _ ∧
     θC' !! γ = Some a ∧
     e' = WrSE (ExprV #a) ∧
     σ' = CState {| χC := χC'; ζC := ζC'; θC := θC'; rootsC := rootsC ρc |} mem').
@@ -56,26 +56,20 @@ Proof using.
                   HγNone & -> & -> & HGCOK' & Hrepr' & Hrootslive' & ?)).
   destruct_and!; simplify_eq.
 
-  assert (χvirt !! γ = None) as Hχvirtγ.
-  { eapply not_elem_of_dom. destruct Hχvirt as [<- _].
+  assert (χ_future !! γ = None) as Hχfutγ.
+  { eapply not_elem_of_dom. destruct Hχfuture as [<- _].
     by eapply not_elem_of_dom. }
-  assert (ζσ !! γ = None) as Hζσγ.
-  { eapply not_elem_of_dom. destruct Hstore_blocks as [HHL HHR].
-    intros (ℓ&Vs&HX1&HX2)%HHR. congruence. }
-  assert (ζvirt !! γ = None) as Hζvirtγ.
-  { eapply not_elem_of_dom. intros H. eapply not_elem_of_dom in Hχvirtγ.
-    apply Hχvirtγ. eapply elem_of_weaken; first done. done. }
+  assert (ζ_future !! γ = None) as Hζfutγ.
+  { eapply not_elem_of_dom. eintros H%elem_of_weaken; last done.
+    by eapply not_elem_of_dom in Hχfutγ. }
   assert (ζC ρc !! γ = None) as HζCγ.
-  { destruct Hfreezeρ as [HL HR]. eapply not_elem_of_dom. rewrite HL.
-    rewrite dom_union_L.
-    intros [HH|HH]%elem_of_union.
-    all: eapply elem_of_dom in HH; destruct HH as [v HHv]; congruence. }
+  { destruct Hζfuture as [HL HR]. eapply not_elem_of_dom. rewrite HL.
+    eapply not_elem_of_dom in Hζfutγ; done. }
 
-  assert (freeze_lstore (<[γ := Bvblock (Mut, blk)]> (ζC ρc)) (ζσ ∪ <[γ:=Bvblock (Mut, blk)]> ζvirt)) as Hfreezeρ_new.
-  { destruct Hfreezeρ as [HfL HfR]; split.
-    - rewrite !dom_insert_L. rewrite dom_union_L in HfL. set_solver+ HfL.
-    - rewrite <- insert_union_r. 2: done.
-      intros γ1 b1 b2 ?%lookup_insert_Some ?%lookup_insert_Some.
+  assert (freeze_lstore (<[γ := Bvblock (Mut, blk)]> (ζC ρc)) (<[γ:=Bvblock (Mut, blk)]> ζ_future)) as Hζfuturenew.
+  { destruct Hζfuture as [HfL HfR]; split.
+    - by rewrite !dom_insert_L HfL.
+    - intros γ1 b1 b2 ?%lookup_insert_Some ?%lookup_insert_Some.
       destruct_or!; destruct_and!; simplify_eq; eauto. }
 
   iMod (set_to_none _ _ _ _ Hpriv with "HσC GCrootspto") as "(HσC&GCrootspto)".
@@ -85,8 +79,8 @@ Proof using.
   iMod (ghost_var_update_halves with "GCχ SIχ") as "(GCχ&SIχ)".
   iMod (ghost_var_update_halves with "GCθ SIθ") as "(GCθ&SIθ)".
 
-  iMod (lstore_own_insert _ γ (Bvblock (Mut, blk)) with "GCζvirt") as "(GCζvirt & Hbp1)". 1: done.
-  iMod (lloc_own_allocate _ γ with "[] GCχvirt") as "(GCχvirt&Hbp2)". 1: done.
+  iMod (lstore_own_insert _ γ (Bvblock (Mut, blk)) with "GCζauth") as "(GCζauth & Hbp1)". 1: done.
+  iMod (lloc_own_allocate _ γ with "[] GCχauth") as "(GCχauth&Hbp2)". 1: done.
 
   do 3 iModIntro. iFrame. cbn -[wrap_prog].
   iSplitL "SIinit". { iExists false. iFrame. }
@@ -96,32 +90,24 @@ Proof using.
   3: iPureIntro; by econstructor.
   2: iFrame; done.
   rewrite /GC /named.
-  iExists _, _, (ζσ), (<[γ:=Bvblock (Mut, blk)]> ζvirt), _, (<[γ:=LlocPrivate]> χvirt).
-  iExists σMLvirt, _, _.
-  rewrite pub_locs_in_lstore_alloc_priv. 2: done. iFrame.
-  cbn. iPureIntro; split_and!; eauto.
-  2: destruct Hstore_blocks as [HsL HsR]; split.
-  - eapply map_disjoint_insert_r. split; done.
-  - intros ℓ Hdom. destruct (HsL ℓ Hdom) as (γ1 & Hγ1). exists γ1. rewrite lookup_insert_ne; first done.
-    intros ->; congruence.
-  - intros γ1; split.
-    + intros (ℓ&Vs&HH1&HH2)%HsR. exists ℓ,Vs; split; try done.
-      rewrite lookup_insert_ne; first done. intros ->; congruence.
-    + intros (ℓ&Vs&[[??]|[??]]%lookup_insert_Some&HH2); try congruence.
-      eapply HsR. by exists ℓ,Vs.
-  - erewrite !dom_insert_L. clear -Hother_blocks. set_solver.
-  - intros ℓ vs γ1 blk1 HH1 [[??]|[? HH2]]%lookup_insert_Some HH3; try congruence.
-    rewrite -!insert_union_r in HH3|-*; try done.
-    rewrite lookup_insert_ne in HH3; last done.
-    specialize (Hstore ℓ vs γ1 blk1 HH1 HH2 HH3).
-    inversion Hstore; subst. econstructor.
-    eapply Forall2_impl; first apply H1.
-    intros vml vl HH4. eapply is_val_mono. 3: apply HH4.
-    + eapply insert_subseteq. done.
-    + eapply insert_subseteq. eapply lookup_union_None; done.
-  - apply expose_llocs_insert_both; eauto.
-  - by apply lloc_map_inj_insert_priv.
-  - eapply GC_correct_transport; done.
+  do 5 iExists _. iFrame.
+  iSplitL "GCσMLv GC_per_loc". 2: iSplit; last iSplit; try iPureIntro.
+  - iExists σMLvirt. iFrame.
+    iPoseProof (GC_per_loc_modify_ζ with "GC_per_loc") as "GC_per_loc".
+    1: apply lloc_map_pubs_lookup_None; by left. unfold named.
+    repeat iSplit; try iPureIntro.
+    * rewrite dom_insert_L; set_solver.
+    * rewrite lloc_map_pubs_insert_priv delete_notin.
+      2: apply lloc_map_pubs_lookup_None; by left. done.
+    * intros ℓ Hℓ; destruct (Hstore _ Hℓ) as (γ'&Hγ'); exists γ'; rewrite lookup_insert_ne; first done.
+      intros ->; simplify_eq.
+  - iExists roots_m. iFrame. iPureIntro; split_and!; try done.
+    by eapply GC_correct_transport.
+  - done.
+  - destruct Hχfuture as (Hf1&Hf2&Hf3); split_and!.
+    * rewrite !dom_insert_L Hf1; done.
+    * by apply lloc_map_inj_insert_priv.
+    * by apply expose_llocs_insert_both; eauto.
 Qed.
 
 End Laws.
