theories/interop/wp_prims/modify.v
@@ -3,7 +3,7 @@ From transfinite.base_logic.lib Require Import ghost_map ghost_var.
 From melocoton Require Import named_props stdpp_extra.
 From melocoton.mlanguage Require Import mlanguage.
 From melocoton.c_interface Require Import defs notation resources.
-From melocoton.interop Require Import state lang basics_resources update_laws.
+From melocoton.interop Require Import state lang basics_resources.
 From melocoton.interop Require Import basics wp_utils.
 From melocoton.interop Require Export prims weakestpre prims_proto.
 From melocoton.interop.wp_prims Require Import common.
@@ -20,6 +20,7 @@ Context `{!wrapperG Σ}.
 
 Implicit Types P : iProp Σ.
 Import mlanguage.
+
 
 Lemma modify_correct e : |- wrap_prog e :: modify_proto.
 Proof using.
@@ -39,60 +40,45 @@ Proof using.
        specialize (HR _ _ _ Hv Helem) as Hinv. inversion Hinv; subst; done. }
 
   iApply wp_pre_cases_c_prim; [done..|].
-  assert (∃ blk', modify_block (Bvblock (Mut, (tg, vs0))) (Z.to_nat i) v' blk')
-    as (blk'&Hblk').
-  { eexists. eapply mk_modify_block. lia. }
+  assert (modify_block (Bvblock (Mut, (tg, vs0))) (Z.to_nat i) v' (Bvblock (Mut, (tg, <[Z.to_nat i:=v']> vs0))))
+    as Hblk'.
+  { eapply mk_modify_block. lia. }
 
   iExists (λ '(e', σ'),
     e' = WrSE (ExprV #0) ∧
-    σ' = CState {| χC := χC ρc; ζC := <[γ:=blk']> (ζC ρc); θC := θC ρc; rootsC := rootsC ρc |} mem).
+    σ' = CState {| χC := χC ρc; ζC := <[γ:=_]> (ζC ρc); θC := θC ρc; rootsC := rootsC ρc |} mem).
   iSplit. { iPureIntro; econstructor; eauto. }
   iIntros (? ? ? (? & ?)); simplify_eq.
 
-  iMod (lstore_own_update _ _ _ blk' with "GCζauth Hpto") as "(GCζvirt&Hpto)".
+  iMod (lstore_own_update with "GCζauth Hpto") as "(GCζvirt&Hpto)".
   iMod (ghost_var_update_halves with "SIζ GCζ") as "(SIζ&GCζ)".
 
-  iPoseProof (GC_per_loc_modify_ζ_in_detail with "GC_per_loc") as "GC_per_loc".
+  inversion Hblk'; simplify_eq.
 
-  iPoseProof (interp_ML_discarded_locs_pub with "GCσMLv GCχNone") as "%Hpublocs".
+  iPoseProof (GC_per_loc_modify_ζ_in_detail with "GC_per_loc") as "GC_per_loc".
+  { erewrite Helem; done. }
   do 3 iModIntro. iFrame. iSplitL "SIinit". { iExists false. iFrame. }
   iApply wp_value; first done.
   change (Z.of_nat 0) with (Z0).
   iApply "Hcont". iFrame.
   iApply ("Cont" with "[-Hpto Hptoacc] [Hpto Hptoacc]").
-  { iExists _, (<[γ:=blk']> (ζσ ∪ ζvirt)), ζσ, (<[γ:=blk']>ζvirt), _, χvirt, σMLvirt.
-    iExists _, _. unfold named. iFrame.
-    erewrite pub_locs_in_lstore_insert_existing; last by eapply elem_of_dom_2. iFrame.
-    iPureIntro; split_and!; eauto; cbn. 1: destruct Hfreezeρ as [HL HR]; split.
-    - by erewrite !dom_insert_L, HL.
-    - intros γ' b1 b2 [[? ?]|[Hne1 H1']]%lookup_insert_Some [[??]|[Hne2 H2']]%lookup_insert_Some; try congruence.
-      1: subst; econstructor.
-      subst. by eapply HR.
-    - rewrite insert_union_r; first done.
-      erewrite map_disjoint_Some_l; done.
-    - eapply map_disjoint_dom. erewrite dom_insert_lookup; last by eexists. by eapply map_disjoint_dom.
-    - rewrite dom_insert_lookup; last by eexists.
-      done.
-    - intros ℓ Vs γ1 bb H1' H2' [[<- <-]|[Hne H3']]%lookup_insert_Some.
-      -- epose proof (map_Forall_lookup_1 _ _ γ ℓ Hpublocs) as Hpub2. cbn in Hpub2.
-         rewrite Hpub2 in H1'; first congruence.
-         eapply pub_locs_in_lstore_lookup; last apply H2'.
-         eapply elem_of_dom_2; done.
-      -- specialize (Hstore _ _ _ _ H1' H2' H3'); inversion Hstore; subst.
-         econstructor. eapply Forall2_impl; first done.
-         intros x' y HH; eapply is_val_insert_immut; last done.
-         1: erewrite lookup_union_r; first done.
-         1: eapply map_disjoint_Some_l; done. done.
-    - split; first apply HGCL.
-      intros γ0 blk1 γ1 Hγ0 [[??]|[Hne1 Hlu]]%lookup_insert_Some Hlloc.
-      2: by eapply HGCR. simplify_eq. inv_modify_block.
-      apply lval_in_vblock, list_insert_lookup_inv in Hlloc as [HLL|HRR];
-        simplify_map_eq.
-      { inv_repr_lval. by eapply elem_of_dom_2. }
-      { eapply HGCR; eauto. 1: rewrite lookup_union_r //.
-        1: eapply map_disjoint_Some_l; eauto. by constructor. } }
-  {  iApply lstore_own_vblock_mutable_as_mut; eauto. iFrame.
-     iSplit. 1: inv_modify_block; simplify_map_eq. 1: iFrame. eauto. }
+  2: { iApply lstore_own_vblock_mutable_as_mut; eauto. iFrame. done. } 
+  do 5 iExists _. iFrame. iSplitR "HSI_GC"; last iSplitL.
+  - iExists _. iFrame. iPureIntro; split_and!; try done.
+    rewrite dom_insert_L subseteq_union_1_L; first done.
+    by eapply singleton_subseteq_l, elem_of_dom_2.
+  - iApply HSI_GC_modify; try done.
+    intros γ' Hinv.
+    inversion Hinv as [?????Hinv']; simplify_eq.
+    apply list_insert_lookup_inv in Hinv' as [Hbef|Hnew].
+    2: simplify_eq; right; by eexists.
+    inversion Hreprw'; simplify_eq.
+    left; by eapply elem_of_dom_2.
+  - iPureIntro. split_and; last done. cbn. destruct Hζfuture as [Hf1 Hf2]; split.
+    1: by rewrite !dom_insert_L Hf1.
+    intros γ' b1 b2 [(Heq&H1)|(Hne&H1)]%lookup_insert_Some H2.
+    + subst γ' b1. rewrite lookup_insert in H2. by simplify_eq.
+    + eapply Hf2; try done. by rewrite lookup_insert_ne in H2.
 Qed.
 
 End Laws.
