theories/interop/wp_prims/write_foreign.v
@@ -23,64 +23,49 @@ Import mlanguage.
 
 Lemma write_foreign_correct e : |- wrap_prog e :: write_foreign_proto.
 Proof using.
-  (* TODO: refactor to share lemmas with prim_modify *)
   iIntros (? ? ? ?) "H". unfold mprogwp. iNamed "H".
   iSplit; first done.
   iIntros (Φ') "Hb Hcont". iApply wp_wrap_call; first done. cbn [snd].
   rewrite weakestpre.wp_unfold. rewrite /weakestpre.wp_pre.
   iIntros "%σ Hσ". cbn -[wrap_prog].
-  SI_at_boundary. iNamed "HGC". SI_GC_agree.
-  iDestruct "Hpto" as "(Hpto & Hsim)".
-  iDestruct (lstore_own_mut_of with "GCζvirt Hpto") as %[Helem _].
+  SI_at_boundary. iNamed "HGC". SI_GC_agree. iNamed "HSI_block_level".
+  iDestruct "Hpto" as "(Hpto & %fid & Hsim)".
+  iPoseProof (lloc_own_foreign_of with "GCχauth Hsim") as "%Hχfgn".
+  iDestruct (lstore_own_mut_of with "GCζauth Hpto") as %[Helem _].
   iAssert ⌜ζC ρc !! γ = Some (Bforeign wo)⌝%I as "%Helem2".
-  { iPureIntro. eapply lookup_union_Some_r in Helem; last apply Hfreezedj.
-    eapply freeze_lstore_lookup_backwards in Helem as (?&Hfrz&?); eauto.
-    inversion Hfrz; by simplify_eq. }
-  destruct HGCOK as [HGCL HGCR]. inv_repr_lval.
+  1: { iPureIntro.
+       destruct Hζfuture as [HL HR].
+       assert (γ ∈ dom (ζC ρc)) as [v Hv]%elem_of_dom by by (rewrite HL; eapply elem_of_dom_2).
+       specialize (HR _ _ _ Hv Helem) as Hinv. inversion Hinv; subst; done. }
 
   iApply wp_pre_cases_c_prim; [done..|].
+
   iExists (λ '(e', σ'),
     e' = WrSE (ExprV #0) ∧
-    σ' = CState (WrapstateC (χC ρc) (<[γ:=Bforeign (Some w')]> (ζC ρc)) (θC ρc) (rootsC ρc)) mem).
+    σ' = CState {| χC := χC ρc; ζC := <[γ:=_]> (ζC ρc); θC := θC ρc; rootsC := rootsC ρc |} mem).
   iSplit. { iPureIntro; econstructor; eauto. }
   iIntros (? ? ? (? & ?)); simplify_eq.
 
-  iMod (lstore_own_update _ _ _ (Bforeign (Some w')) with "GCζvirt Hpto") as "(GCζvirt&Hpto)".
+  iMod (lstore_own_update with "GCζauth Hpto") as "(GCζvirt&Hpto)".
   iMod (ghost_var_update_halves with "SIζ GCζ") as "(SIζ&GCζ)".
-  iPoseProof (interp_ML_discarded_locs_pub with "GCσMLv GCχNone") as "%Hpublocs".
-  do 3 iModIntro. iFrame. cbn -[wrap_prog] in *.
-  iSplitL "SIinit". { iExists false. iFrame. }
+  iPoseProof (GC_per_loc_modify_ζ with "GC_per_loc") as "GC_per_loc".
+  { eapply lloc_map_pubs_lookup_None. do 2 right. by eexists. }
+  do 3 iModIntro. iFrame. iSplitL "SIinit". { iExists false. iFrame. }
   iApply wp_value; first done.
   change (Z.of_nat 0) with (Z0).
   iApply "Hcont". iFrame.
-  iApply ("Cont" with "[-Hpto Hsim] [$Hpto $Hsim]").
-  { iExists _, (<[γ:=Bforeign (Some w')]> (ζσ ∪ ζvirt)), ζσ, (<[γ:=Bforeign (Some w')]>ζvirt), _, χvirt, σMLvirt.
-    iExists _, _. unfold named. iFrame.
-    erewrite pub_locs_in_lstore_insert_existing; last by eapply elem_of_dom_2. iFrame.
-    iPureIntro; split_and!; eauto; cbn. 1: destruct Hfreezeρ as [HL HR]; split.
-    - by erewrite !dom_insert_L, HL.
-    - intros γ' b1 b2 [[? ?]|[Hne1 H1']]%lookup_insert_Some [[??]|[Hne2 H2']]%lookup_insert_Some; try congruence.
-      1: subst; econstructor.
-      subst. by eapply HR.
-    - rewrite insert_union_r; first done.
-      erewrite map_disjoint_Some_l; done.
-    - eapply map_disjoint_dom. erewrite dom_insert_lookup; last by eexists. by eapply map_disjoint_dom.
-    - rewrite dom_insert_lookup; last by eexists.
-      done.
-    - intros ℓ Vs γ1 bb H1' H2' [[<- <-]|[Hne H3']]%lookup_insert_Some.
-      -- epose proof (map_Forall_lookup_1 _ _ γ ℓ Hpublocs) as Hpub2. cbn in Hpub2.
-         rewrite Hpub2 in H1'; first congruence.
-         eapply pub_locs_in_lstore_lookup; last apply H2'.
-         eapply elem_of_dom_2; done.
-      -- specialize (Hstore _ _ _ _ H1' H2' H3'); inversion Hstore; subst.
-         econstructor. eapply Forall2_impl; first done.
-         intros x' y HH; eapply is_val_insert_immut; last done.
-         1: erewrite lookup_union_r; first done.
-         1: eapply map_disjoint_Some_l; done. done.
-    - split; first apply HGCL.
-      intros γ0 blk1 γ1 Hγ0 [[??]|[Hne1 Hlu]]%lookup_insert_Some Hlloc.
-      2: by eapply HGCR. simplify_eq. inversion Hlloc. }
-  { done. }
+  iApply ("Cont" with "[-Hpto Hsim] [$Hpto Hsim]").
+  2: { iSplit; first done. by iExists _. } 
+  do 5 iExists _. iFrame. iSplitR "HSI_GC"; last iSplitL.
+  - iExists _. iFrame. iPureIntro; split_and!; try done.
+    rewrite dom_insert_L subseteq_union_1_L; first done.
+    by eapply singleton_subseteq_l, elem_of_dom_2.
+  - iApply HSI_GC_modify; try done. intros ?; inversion 1.
+  - iPureIntro. split_and; last done. cbn. destruct Hζfuture as [Hf1 Hf2]; split.
+    1: by rewrite !dom_insert_L Hf1.
+    intros γ' b1 b2 [(Heq&H1)|(Hne&H1)]%lookup_insert_Some H2.
+    + subst γ' b1. rewrite lookup_insert in H2. by simplify_eq.
+    + eapply Hf2; try done. by rewrite lookup_insert_ne in H2.
 Qed.
 
 End Laws.
